experiment/Experiment.Steel.Repr.ST_to_SF.Base.fsti
@@ -14,27 +14,6 @@ open Experiment.Steel.Repr.SF
 
 #set-options "--fuel 1 --ifuel 1"
 
-(* ST.seq_sel_eq written with a conjunction instead of a forall *)
-let rec seq_sel_eq_eff_aux (#pre #post : Fl.ty_list) (f_eq : M.veq_eq_t (L.length pre) (L.length post))
-                           (sl0 : Fl.flist pre) (sl1 : Fl.flist post) (i : nat)
-  : Pure prop (requires M.veq_typ_eq pre post f_eq) (ensures fun _ -> True) (decreases L.length post - i)
-  = if i >= L.length post then True
-    else match f_eq i with
-    | None   -> seq_sel_eq_eff_aux f_eq sl0 sl1 (i+1)
-    | Some j -> sl1 i == U.cast _ (sl0 j) /\ seq_sel_eq_eff_aux f_eq sl0 sl1 (i+1)
-
-let seq_sel_eq_eff (#pre #post : Fl.ty_list) (f_eq : M.veq_eq_t (L.length pre) (L.length post))
-                   (sl0 : Fl.flist pre) (sl1 : Fl.flist post)
-  : Pure prop (requires M.veq_typ_eq pre post f_eq) (ensures fun _ -> True)
-  = seq_sel_eq_eff_aux f_eq sl0 sl1 0
-
-val seq_sel_eq_eff_sound
-      (#pre #post : Fl.ty_list) (f_eq : M.veq_eq_t (L.length pre) (L.length post))
-      (sl0 : Fl.flist pre) (sl1 : Fl.flist post)
-  : Lemma (requires M.veq_typ_eq pre post f_eq)
-          (ensures  seq_sel_eq_eff f_eq sl0 sl1 <==> ST.seq_sel_eq f_eq sl0 sl1)
-
-
 [@@ strict_on_arguments [3]] (* strict on t *)
 let rec repr_SF_of_ST
       (#a : Type u#a) (#pre : ST.pre_t u#b) (#post : ST.post_t u#a u#b a)
@@ -44,7 +23,7 @@ let rec repr_SF_of_ST
   | ST.Tequiv pre post0 e ->
           // TODO? specialized constructor / wp
           Tspec U.unit' (const_post post0) (e.seq_req sl0)
-                (fun _ sl1 -> seq_sel_eq_eff e.seq_eq sl0 sl1 /\ e.seq_ens sl0 sl1)
+                (fun _ sl1 -> M.veq_sel_eq_eff e.seq_eq sl0 sl1 /\ e.seq_ens sl0 sl1)
   | ST.Tframe a pre post frame f ->
           let (sl0', sl_frame) = Fl.splitAt_ty pre frame sl0 in
           Tbind a a _ _ (repr_SF_of_ST f sl0') (fun x sl1' ->
